template-coq/src/constr_quoter.ml
@@ -61,6 +61,7 @@ struct
 
   let pkg_datatypes = ["Coq";"Init";"Datatypes"]
   let pkg_string = ["Coq";"Strings";"String"]
+  let pkg_base_reify = ["Template";"BasicAst"]
   let pkg_reify = ["Template";"Ast"]
   let pkg_template_monad = ["Template";"TemplateMonad"]
   let pkg_univ = ["Template";"kernel";"univ"]
@@ -68,6 +69,7 @@ struct
   let pkg_ugraph = ["Template";"kernel";"uGraph"]
   let ext_pkg_univ s = List.append pkg_univ [s]
 
+  let r_base_reify = resolve_symbol pkg_base_reify
   let r_reify = resolve_symbol pkg_reify
   let r_template_monad = resolve_symbol pkg_template_monad
   let r_template_monad_p = resolve_symbol_p pkg_template_monad
@@ -96,22 +98,22 @@ struct
   let pair a b f s = Constr.mkApp (c_pair, [| a ; b ; f ; s |])
 
     (* reify the constructors in Template.Ast.v, which are the building blocks of reified terms *)
-  let nAnon = r_reify "nAnon"
-  let nNamed = r_reify "nNamed"
-  let kVmCast = r_reify "VmCast"
-  let kNative = r_reify "NativeCast"
-  let kCast = r_reify "Cast"
-  let kRevertCast = r_reify "RevertCast"
+  let nAnon = r_base_reify "nAnon"
+  let nNamed = r_base_reify "nNamed"
+  let kVmCast = r_base_reify "VmCast"
+  let kNative = r_base_reify "NativeCast"
+  let kCast = r_base_reify "Cast"
+  let kRevertCast = r_base_reify "RevertCast"
   let lProp = resolve_symbol pkg_level "lProp"
   let lSet = resolve_symbol pkg_level "lSet"
-  let sfProp = r_reify "InProp"
-  let sfSet = r_reify "InSet"
-  let sfType = r_reify "InType"
-  let tident = r_reify "ident"
-  let tname = r_reify "name"
-  let tIndTy = r_reify "inductive"
-  let tmkInd = r_reify "mkInd"
-  let tsort_family = r_reify "sort_family"
+  let sfProp = r_base_reify "InProp"
+  let sfSet = r_base_reify "InSet"
+  let sfType = r_base_reify "InType"
+  let tident = r_base_reify "ident"
+  let tname = r_base_reify "name"
+  let tIndTy = r_base_reify "inductive"
+  let tmkInd = r_base_reify "mkInd"
+  let tsort_family = r_base_reify "sort_family"
   let tmkdecl = r_reify "mkdecl"
   let (tTerm,tRel,tVar,tMeta,tEvar,tSort,tCast,tProd,
        tLambda,tLetIn,tApp,tCase,tFix,tConstructor,tConst,tInd,tCoFix,tProj) =
@@ -137,7 +139,7 @@ struct
   let tinit_graph = resolve_symbol pkg_ugraph "init_graph"
   let tadd_global_constraints = resolve_symbol pkg_ugraph  "add_global_constraints"
 
-  let (tdef,tmkdef) = (r_reify "def", r_reify "mkdef")
+  let (tdef,tmkdef) = (r_base_reify "def", r_base_reify "mkdef")
   let (tLocalDef,tLocalAssum,tlocal_entry) = (r_reify "LocalDef", r_reify "LocalAssum", r_reify "local_entry")
 
   let (cFinite,cCoFinite,cBiFinite) = (r_reify "Finite", r_reify "CoFinite", r_reify "BiFinite")
@@ -165,7 +167,8 @@ struct
 
   let (tcbv, tcbn, thnf, tall, tlazy, tunfold) = (r_template_monad "cbv", r_template_monad "cbn", r_template_monad "hnf", r_template_monad "all", r_template_monad "lazy", r_template_monad "unfold")
 
-  let (tglobal_reference, tConstRef, tIndRef, tConstructRef) = (r_reify "global_reference", r_reify "ConstRef", r_reify "IndRef", r_reify "ConstructRef")
+  let (tglobal_reference, tConstRef, tIndRef, tConstructRef) =
+    (r_base_reify "global_reference", r_base_reify "ConstRef", r_base_reify "IndRef", r_base_reify "ConstructRef")
 
   let (tmReturn, tmBind, tmQuote, tmQuoteRec, tmEval, tmDefinition, tmAxiom, tmLemma, tmFreshName, tmAbout, tmCurrentModPath,
        tmMkDefinition, tmMkInductive, tmPrint, tmFail, tmQuoteInductive, tmQuoteConstant, tmQuoteUniverses, tmUnquote, tmUnquoteTyped, tmInferInstance, tmExistingInstance) =
