extraction/theories/EAst.v
@@ -4,7 +4,7 @@ Require Import Coq.Strings.String.
 Require Import Coq.PArith.BinPos.
 Require Import List. Import ListNotations.
 From Template Require Import monad_utils.
-From Template Require Export Ast.
+From Template Require Export BasicAst.
 
 (** Extracted terms
 
