pcuic/theories/PCUICRetyping.v
@@ -1,7 +1,7 @@
 (* Distributed under the terms of the MIT license.   *)
 
 From Coq Require Import Bool String List Program BinPos Compare_dec Omega.
-From Template Require Import config monad_utils utils Ast univ.
+From Template Require Import config monad_utils utils BasicAst univ.
 From PCUIC Require Import PCUICAst PCUICAstUtils PCUICInduction PCUICLiftSubst PCUICUnivSubst PCUICTyping PCUICChecker.
 Require Import String.
 Local Open Scope string_scope.
