pcuic/theories/PCUICWeakening.v
@@ -1,7 +1,7 @@
 (* Distributed under the terms of the MIT license.   *)
 
 From Coq Require Import Bool String List Program BinPos Compare_dec Omega Lia.
-From Template Require Import config utils Ast.
+From Template Require Import config utils BasicAst.
 From PCUIC Require Import PCUICAst PCUICAstUtils PCUICInduction PCUICLiftSubst PCUICUnivSubst PCUICTyping PCUICWeakeningEnv PCUICClosed.
 Require Import ssreflect ssrbool.
 
