pcuic/theories/PCUICWeakeningEnv.v
@@ -1,7 +1,7 @@
 (* Distributed under the terms of the MIT license.   *)
 
 From Coq Require Import Bool String List Program BinPos Compare_dec Arith Lia.
-From Template Require Import config utils Ast AstUtils.
+From Template Require Import config utils BasicAst AstUtils.
 From PCUIC Require Import PCUICAst PCUICAstUtils PCUICInduction PCUICLiftSubst PCUICUnivSubst PCUICTyping.
 Require Import ssreflect ssrbool.
 
