template-coq/theories/BasicAst.v
@@ -1,0 +1,51 @@
+(* Distributed under the terms of the MIT license.   *)
+Require Import Coq.Strings.String.
+
+Definition ident := string. (* e.g. nat *)
+Definition kername := string. (* e.g. Coq.Init.Datatypes.nat *)
+
+Inductive name : Set :=
+| nAnon
+| nNamed (_ : ident).
+
+Record inductive : Set := mkInd { inductive_mind : kername ;
+                                  inductive_ind : nat }.
+Arguments mkInd _%string _%nat.
+
+Definition projection : Set := inductive * nat (* params *) * nat (* argument *).
+
+(** Parametrized by term because term is not yet defined *)
+
+Record def (term : Set) : Set := mkdef {
+  dname : name; (* the name **)
+  dtype : term;
+  dbody : term; (* the body (a lambda term). Note, this may mention other (mutually-defined) names **)
+  rarg  : nat  (* the index of the recursive argument, 0 for cofixpoints **) }.
+
+Arguments dname {term} _.
+Arguments dtype {term} _.
+Arguments dbody {term} _.
+Arguments rarg {term} _.
+
+Definition mfixpoint (term : Set) : Set :=
+  list (def term).
+
+(** Sort families *)
+
+Inductive sort_family : Set := InProp | InSet | InType.
+
+(** The kind of a cast *)
+
+Inductive cast_kind : Set :=
+| VmCast
+| NativeCast
+| Cast
+| RevertCast.
+
+(** Kernel declaration references [global_reference] *)
+
+Inductive global_reference :=
+(* VarRef of Names.variable *)
+| ConstRef : kername -> global_reference
+| IndRef : inductive -> global_reference
+| ConstructRef : inductive -> nat -> global_reference.
